Coq/src/drf/DRF_SC.v
@@ -17,22 +17,22 @@ Require Import DRF_RLX.
 Set Implicit Arguments.
 
 Theorem drf_rc11_sc P S X
-      (RA_RACE_FREE : SC_RA_race_free_program P)
+      (RA_RACE_FREE : sc_ra_race_free_program P)
       (EXEC : program_execution P S X)
-      (RC11 : rc11_consistent_x S X) :
-  sc_consistent_x S X.
+      (RC11 : rc11_consistent_ex S X) :
+  sc_consistent_ex S X.
 Proof.
 Admitted.
 
 Theorem drf_sc P S X
         (nInitProg : ~ IdentMap.In tid_init P)
-        (RA_RACE_FREE : SC_RA_race_free_program P)
+        (RA_RACE_FREE : sc_ra_race_free_program P)
         (EXEC : program_execution P S X) :
-  sc_consistent_x S X.
+  sc_consistent_ex S X.
 Proof.
   eapply drf_rc11_sc; eauto.
   eapply drf_rlx; eauto.
   red. intros S' X' EXEC' RC11.
-  apply RA_race_free_in_RLX_race_free, RA_RACE_FREE; auto.
+  apply ra_race_free_in_rlx_race_free, RA_RACE_FREE; auto.
   eby eapply drf_rc11_sc.
 Qed.
